init array

dp/lis.dfy
@@ -16,40 +16,68 @@ reads x, y
     multiset(y[..]) * multiset(x[..]) == multiset(x[..])
 }
 
+predicate boundedElements(x: array<nat>) 
+reads x
+{
+    forall i :: 0 <= i < x.Length ==> 0 < x[i] <= x.Length
+}
+
+predicate uniformArray(x: array<nat>) 
+reads x
+{
+    forall i, j :: 0 <= i < j < x.Length ==> x[i] == x[j]
+}
+
+method initLIS(x: array<nat>, val: nat) 
+requires 0 < val <= x.Length
+ensures uniformArray(x) 
+ensures boundedElements(x)
+modifies x
+{
+    forall i | 0 <= i < x.Length 
+    {
+        x[i] := val;
+    }
+}
+
 method computeLIS(a: array<int>) returns (lisN: nat) 
 requires a.Length > 0
 ensures 0 <= lisN <= a.Length
 {
     var n := a.Length;
-    if n < 3 { return 1; }
-    if n == 0 { return 0; }
-
     var lis := new nat[n];
-    var i, j := 1, 1;
+    initLIS(lis, 1);
 
-    while i < n 
-    invariant 0 < j <= i <= n
+    var i, j := 0, 0;
+
+    assert lis.Length == n;
+
+    while i < n
+    invariant 0 <= j <= i <= n
+    invariant boundedElements(lis)
     decreases n - i 
     {
-        lis[i] := 1;
-
         while j < i - 1 
-        invariant 0 < j <= i
+        invariant 0 <= j <= i
         decreases i - j - 1 
         {
-            if a[j] < a[i] && lis[i] < lis[j] {
+            /*
+            if a[j] < a[i] && lis[i] < 1 + lis[j] {
                 lis[i] := 1 + lis[j];
             }
+            */
             j := j + 1;
         }
         i := i + 1;
     }
 
-    var max := 1;
-    var k := 2;
+    assert lis.Length <= n;
+
+    var max := 0;
+    var k := 1;
 
     while k < n
-    invariant 0 < max <= k <= n
+    invariant  0 <= max < k <= n
     decreases n - k 
     {
         if lis[k] > lis[max] {
@@ -58,9 +86,11 @@ ensures 0 <= lisN <= a.Length
         k := k + 1;
     }
 
-    assert max > 0;
-    assert max <= lis.Length;
-   //assert increasing(lis);
+    assert max < lis.Length;
+    assert max >= 0;
 
-    return lis[max];
+    lisN := lis[max];
+    assert 0 <= lisN <= n;
+
+    return lisN;
 }
